working zwischenstand

FiLProject/Tree23/Delete.lean
@@ -21,6 +21,7 @@ def deleteTree : DeleteUp α → Tree23 α
 | DeleteUp.eq t => t
 | DeleteUp.underflow t => t
 
+@[grind]
 def node21 : DeleteUp α → α → (t: Tree23 α) → t ≠ nil → DeleteUp α
 | DeleteUp.eq t₁, a, t₂, _ => DeleteUp.eq (Tree23.node2 t₁ a t₂)
 | DeleteUp.underflow t₁, a, r, h =>
@@ -35,6 +36,7 @@ def node21 : DeleteUp α → α → (t: Tree23 α) → t ≠ nil → DeleteUp α
       -- the top element to the left, making both sides equal height
       DeleteUp.eq (Tree23.node2 (Tree23.node2 t₁ a t₂) b (Tree23.node2 t₃ c t₄))
 
+@[grind]
 def node22 : (t: Tree23 α) → α → DeleteUp α → t ≠ nil → DeleteUp α
 | t₁, a, DeleteUp.eq t₂, _ => DeleteUp.eq (Tree23.node2 t₁ a t₂)
 | l, a, DeleteUp.underflow t_r, h =>
@@ -45,6 +47,7 @@ def node22 : (t: Tree23 α) → α → DeleteUp α → t ≠ nil → DeleteUp α
     | node3 t₁ b t₂ c t₃ =>
       DeleteUp.eq (Tree23.node2 (Tree23.node2 t₁ b t₂) c (Tree23.node2 t₃ a t_r))
 
+@[grind]
 def node31 : DeleteUp α → α → (t₁ : Tree23 α) → α → (t₂ : Tree23 α) → t₁ ≠ nil → t₂ ≠ nil → DeleteUp α
 | DeleteUp.eq t₁, a, t₂, b, t₃, _, _ => DeleteUp.eq (Tree23.node3 t₁ a t₂ b t₃)
 | DeleteUp.underflow t₁, a, t_m, c, r, _, _ =>
@@ -53,6 +56,7 @@ def node31 : DeleteUp α → α → (t₁ : Tree23 α) → α → (t₂ : Tree23
     | node2 t₂ b t₃ => DeleteUp.eq (Tree23.node2 (Tree23.node3 t₁ a t₂ b t₃) c r)
     | node3 t₂ b t₃ c_inner t₄ => DeleteUp.eq (node3 (node2 t₁ a t₂) b (node2 t₃ c_inner t₄) c r)
 
+@[grind]
 def node32 : (t₁ : Tree23 α) → α → DeleteUp α → α → (t₂ : Tree23 α) →  t₁ ≠ nil → t₂ ≠ nil → DeleteUp α
 | t₁, a, DeleteUp.eq t₂, b, t₃, _, _ =>  DeleteUp.eq (node3 t₁ a t₂ b t₃)
 | t₁, a, DeleteUp.underflow t₂, b, t_r, _, _ =>
@@ -61,6 +65,7 @@ def node32 : (t₁ : Tree23 α) → α → DeleteUp α → α → (t₂ : Tree23
     | node2 t₃ c t₄ => DeleteUp.eq (node2 t₁ a (node3 t₂ b t₃ c t₄))
     | node3 t₃ c t₄ d t₅ => DeleteUp.eq (node3 t₁ a (node2 t₂ b t₃) c (node2 t₄ d t₅))
 
+@[grind]
 def node33 : (t₁ : Tree23 α) → α → (t₂ : Tree23 α) → α → DeleteUp α →  t₁ ≠ nil → t₂ ≠ nil → DeleteUp α
 | t₁, a, t₂, b, DeleteUp.eq t₃, _, _ => DeleteUp.eq (node3 t₁ a t₂ b t₃)
 | t₁, a, t_m, c, DeleteUp.underflow t_u, _, _ =>
@@ -71,21 +76,21 @@ def node33 : (t₁ : Tree23 α) → α → (t₂ : Tree23 α) → α → DeleteU
 
 @[grind]
 def splitMin : (t : Tree23 α) → complete t → t ≠ nil → α × DeleteUp α
-| nil, _, h => by grind[complete]
+| nil, _, h => by grind
 | node2 l a r, hc, _ =>
   if h: l = nil then
     (a, DeleteUp.underflow nil)
   else
     -- extract the smallest element merge reduced left side with right side
     -- ah, that is why this is called splitMin ...
-    let (x, l') := splitMin l (by grind[complete]) (by assumption)
+    let (x, l') := splitMin l (by grind  ) (by assumption)
     have hr : r ≠ nil := by grind[height_pos_not_nil, complete]
     (x, node21 l' a r (by assumption))
 | node3 l a m b r, _, _ =>
   if h: l = nil then
     (a, DeleteUp.eq (node2 nil b nil))
   else
-    let (x, l') := splitMin l (by grind[complete]) (by assumption)
+    let (x, l') := splitMin l (by grind  ) (by assumption)
     have hr : r ≠ nil := by grind[height_pos_not_nil, complete]
     have hm : m ≠ nil := by grind[height_pos_not_nil, complete]
     (x, node31 l' a m b r (by assumption) (by assumption))
@@ -103,17 +108,17 @@ def del : α → (t : Tree23 α) →  complete t → DeleteUp α
       DeleteUp.eq (Tree23.node2 Tree23.nil a Tree23.nil)
   else
     -- not leaf, so l and r are both not nil
-    have h2 : r ≠ nil := by grind[complete]
+    have h2 : r ≠ nil := by grind
 
     if (x < a) then
       -- recursion on left subtree and handle underflow logic via node21
-      node21 (del x l (by grind[complete])) a r (by assumption)
+      node21 (del x l (by grind  )) a r (by assumption)
     else if (x = a) then
-      let (a0, r0) := splitMin r (by grind[complete]) (by assumption)
+      let (a0, r0) := splitMin r (by grind  ) (by assumption)
       node22 l a0 r0 (by assumption)
     else
       -- recursion on right subtree and handle underflow logic via node22
-      node22 l a (del x r (by grind[complete])) (by assumption)
+      node22 l a (del x r (by grind  )) (by assumption)
 | x, node3 l a m b r, h =>
   if hl: l = Tree23.nil then
     DeleteUp.eq (if x = a then
@@ -124,26 +129,27 @@ def del : α → (t : Tree23 α) →  complete t → DeleteUp α
       Tree23.node3 Tree23.nil a Tree23.nil b Tree23.nil
     )
   else
-    have hr : r ≠ nil := by grind[complete]
-    have hm : m ≠ nil := by grind[complete]
+    have hr : r ≠ nil := by grind
+    have hm : m ≠ nil := by grind
 
     if (x < a) then
-      node31 (del x l (by grind[complete])) a m b r (by assumption) (by assumption)
+      node31 (del x l (by grind  )) a m b r (by assumption) (by assumption)
     else if (x = a) then
-      let (a', m') := splitMin m (by grind[complete]) (by assumption)
+      let (a', m') := splitMin m (by grind  ) (by assumption)
       node32 l a' m' b r (by assumption) (by assumption)
     else
       if (x < b) then
-        node32 l a (del x m (by grind[complete])) b r (by assumption) (by assumption)
+        node32 l a (del x m (by grind  )) b r (by assumption) (by assumption)
       else if (x = b) then
-        let (b', r') := splitMin r (by grind[complete]) (by assumption)
+        let (b', r') := splitMin r (by grind  ) (by assumption)
         node33 l a m b' r' (by assumption) (by assumption)
       else
-        node33 l a m b (del x r (by grind[complete])) (by assumption) (by assumption)
+        node33 l a m b (del x r (by grind  )) (by assumption) (by assumption)
 
 def delete (x : α) (t : Tree23 α) (hc : complete t) : Tree23 α :=
   deleteTree (del x t hc)
 
+@[grind]
 def deleteHeight : DeleteUp α → ℕ
 | DeleteUp.eq t => height t
 | DeleteUp.underflow t => height t + 1
@@ -155,10 +161,10 @@ lemma completeness_preservation_deleteTree_node21 (a : α) (r : Tree23 α) (l' :
   (hheight : height r = deleteHeight l' ) (hrn : r ≠ nil) :
     complete (deleteTree (node21 l' a r hrn)) := by
   induction l' with
-  | eq l => grind[complete, node21, deleteHeight]
+  | eq l => grind
   | underflow l =>
     unfold node21
-    grind[complete, deleteHeight, complete]
+    grind
 
 omit [LinearOrder α] in
 lemma completeness_preservation_deleteTree_node22 (a : α) (l : Tree23 α) (r' : DeleteUp α)
@@ -166,10 +172,10 @@ lemma completeness_preservation_deleteTree_node22 (a : α) (l : Tree23 α) (r' :
   (hheight : height l = deleteHeight r' ) (hln : l ≠ nil) :
     complete (deleteTree (node22 l a r' hln)) := by
   induction r' with
-  | eq r => grind[complete, node22, deleteHeight]
+  | eq r => grind
   | underflow r =>
     unfold node22
-    grind[complete, deleteHeight, complete]
+    grind
 
 omit [LinearOrder α] in
 lemma completeness_preservation_deleteTree_node31 (a b : α) (m r : Tree23 α) (l' : DeleteUp α)
@@ -177,10 +183,10 @@ lemma completeness_preservation_deleteTree_node31 (a b : α) (m r : Tree23 α) (
   (hhrl' : height r = deleteHeight l') (hhmr : height m = height r) (hrn : r ≠ nil) (hmn : m ≠ nil):
     complete (deleteTree (node31 l' a m b r hmn hrn)) := by
   induction l' with
-  | eq l => grind[complete, node31, deleteHeight]
+  | eq l => grind
   | underflow l =>
     unfold node31
-    grind[complete, deleteHeight, complete]
+    grind
 
 omit [LinearOrder α] in
 lemma completeness_preservation_deleteTree_node32 (a b : α) (l r : Tree23 α) (m' : DeleteUp α)
@@ -188,10 +194,10 @@ lemma completeness_preservation_deleteTree_node32 (a b : α) (l r : Tree23 α) (
   (hhrm' : height r = deleteHeight m') (hhlr : height l = height r) (hln : l ≠ nil) (hrn : r ≠ nil):
     complete (deleteTree (node32 l a m' b r hln hrn)) := by
   induction m' with
-  | eq m => grind[complete, node32, deleteHeight]
+  | eq m => grind
   | underflow m =>
     unfold node32
-    grind[complete, deleteHeight, complete]
+    grind
 
 omit [LinearOrder α] in
 lemma completeness_preservation_deleteTree_node33 (a b : α) (l m : Tree23 α) (r' : DeleteUp α)
@@ -199,17 +205,17 @@ lemma completeness_preservation_deleteTree_node33 (a b : α) (l m : Tree23 α) (
   (hhlr' : height l = deleteHeight r') (hhlm : height l = height m) (hln : l ≠ nil) (hmn : m  ≠ nil):
     complete (deleteTree (node33 l a m b r' hln hmn)) := by
   induction r' with
-  | eq r => grind[complete, node33, deleteHeight]
+  | eq r => grind
   | underflow r =>
     unfold node33
-    grind[complete, deleteHeight, complete]
+    grind
 
 omit [LinearOrder α] in
 lemma max_height_node21 (a : α) (r : Tree23 α)  (l' : DeleteUp α) (h : 0 < height r):
     deleteHeight (node21 l' a r (by grind[height_pos_not_nil])) = max (deleteHeight l') (height r) + 1 := by
   unfold deleteHeight
   cases l' with
-  | eq l => grind[node21]
+  | eq l => grind
   | underflow t =>
     simp[node21]
     grind
@@ -219,7 +225,7 @@ lemma max_height_node22 (a : α) (l : Tree23 α)  (r' : DeleteUp α) (h : 0 < he
     deleteHeight (node22 l a r' (by grind[height_pos_not_nil])) = max (deleteHeight r') (height l) + 1 := by
   unfold deleteHeight
   cases r' with
-  | eq l => grind[node22]
+  | eq l => grind
   | underflow t =>
     simp[node22]
     grind
@@ -229,7 +235,7 @@ lemma max_height_node31 (a b : α) (m r : Tree23 α) (l' : DeleteUp α) (hr : 0 
     deleteHeight (node31 l' a m b r (by grind[height_pos_not_nil]) (by grind[height_pos_not_nil])) = max (deleteHeight l') (max (height m) (height r)) + 1 := by
   unfold deleteHeight
   cases l' with
-  | eq t => grind[node31]
+  | eq t => grind
   | underflow t =>
     simp[node31]
     grind
@@ -239,7 +245,7 @@ lemma max_height_node32 (a b : α) (l r : Tree23 α) (m' : DeleteUp α) (hl : 0 
     deleteHeight (node32 l a m' b r (by grind[height_pos_not_nil]) (by grind[height_pos_not_nil])) = max (deleteHeight m') (max (height l) (height r)) + 1 := by
   unfold deleteHeight
   cases m' with
-  | eq t => grind[node32]
+  | eq t => grind
   | underflow t =>
     simp[node32]
     grind
@@ -249,13 +255,10 @@ lemma max_height_node33 (a b : α) (l m : Tree23 α) (r' : DeleteUp α) (hl : 0 
     deleteHeight (node33 l a m b r' (by grind[height_pos_not_nil]) (by grind[height_pos_not_nil])) = max (deleteHeight r') (max (height l) (height m)) + 1 := by
   unfold deleteHeight
   cases r' with
-  | eq t => grind[node33]
+  | eq t => grind
   | underflow t =>
     simp[node33]
-    cases m with
-    | nil => grind
-    | node2 lm am rm => grind
-    | node3 l a m b r => grind
+    cases m <;> grind
 
 lemma splitMin_height_complete (t : Tree23 α )
   (hct: complete t) (hht : 0 < height t) :
@@ -264,100 +267,88 @@ lemma splitMin_height_complete (t : Tree23 α )
   | nil => grind
   | node2 l a r l_ih r_ih =>
     by_cases h : l = nil
-    · grind[deleteHeight, height_pos_not_nil, complete]
-    · grind[max_height_node21, complete]
+    · grind
+    · grind[max_height_node21]
   | node3 l a m b r l_ih m_ih r_ih =>
     by_cases h : l = nil
-    · grind[deleteHeight, height_pos_not_nil, complete]
-    · grind[ max_height_node31, complete]
+    · grind
+    · grind[ max_height_node31]
 
 lemma splitMin_complete (t : Tree23 α)
   (hct : complete t) (hht : 0 < height t) :
     complete (deleteTree (splitMin t hct (by grind[height_pos_not_nil])).2) := by
   induction t with
-  | nil => grind[complete]
+  | nil => grind
   | node2 l a r l_ih r_ih =>
       by_cases h : l = nil
-      · grind[complete]
-      · grind[completeness_preservation_deleteTree_node21, complete, splitMin_height_complete]
+      · grind
+      · grind[completeness_preservation_deleteTree_node21, splitMin_height_complete]
   | node3 l a m a r l_ih m_ih r_ih =>
       by_cases h : l = nil
-      · grind[complete]
-      · grind[completeness_preservation_deleteTree_node31, complete, splitMin_height_complete]
+      · grind
+      · grind[completeness_preservation_deleteTree_node31,splitMin_height_complete]
 
 lemma complete_deleteHeight (t : Tree23 α) (x : α) (h : complete t):
     deleteHeight (del x t (by assumption)) = height t := by
   induction t with
-  | nil => grind[del, deleteHeight]
+  | nil => grind[del]
   | node2 l a r l_ih r_ih =>
     unfold del
     split
-    · grind[deleteHeight, complete]
+    · grind
     · split
-      · expose_names
-        rw[max_height_node21]
-        · grind
-        · grind[complete]
+      · grind[max_height_node21]
       · split
         · expose_names
           rw[max_height_node22]
           · have hr: r ≠ nil := by grind[complete, height]
-            have : deleteHeight (splitMin r (by grind[complete]) hr).2 = height r := by
+            have : deleteHeight (splitMin r (by grind  ) hr).2 = height r := by
               rw[splitMin_height_complete]
               grind
             grind[deleteHeight, complete]
-          · grind[complete]
-        · expose_names
-          rw[max_height_node22]
           · grind
-          · grind[complete]
+        · grind[max_height_node22]
   | node3 l a m b r l_ih m_ih r_ih =>
     unfold del
     -- aesop (add norm [deleteHeight, complete, splitMin, splitMin_height_complete, max_height_node31, max_height_node32, max_height_node33] )
     split
-    · grind[deleteHeight, complete]
+    · grind
     · split
-      · rw[max_height_node31]
-        · grind[height]
-        · grind[complete]
-        · grind[complete]
+      · grind[max_height_node31]
       · split
         · rw[max_height_node32]
-          · have hm : m ≠ nil := by grind[complete]
-            have : deleteHeight (splitMin m (by grind[complete]) hm).2 = height m := by
+          · have hm : m ≠ nil := by grind
+            have : deleteHeight (splitMin m (by grind) hm).2 = height m := by
               rw[splitMin_height_complete]
               grind
-            grind[deleteHeight, complete]
-          · grind[complete]
-          · grind[complete]
+            grind
+          · grind
+          · grind
         · split
-          · rw[max_height_node32]
-            · grind
-            · grind[complete]
-            · grind[complete]
+          · grind[max_height_node32]
           · split
             · rw[max_height_node33]
-              have hr: r ≠ nil := by grind[complete]
-              have : deleteHeight (splitMin r (by grind[complete]) hr).2 = height r := by
+              have hr: r ≠ nil := by grind
+              have : deleteHeight (splitMin r (by grind  ) hr).2 = height r := by
                 rw[splitMin_height_complete]
                 grind
-              grind[height, deleteHeight, complete]
-              · grind[complete]
-              · grind[complete]
+              grind
+              · grind
+              · grind
             · rw[max_height_node33]
               · grind
-              · grind[complete]
-              · grind[complete]
+              · grind
+              · grind
 
 
 lemma complete_complete_del (t : Tree23 α) (x : α) (h : complete t):
     complete (deleteTree (del x t h)) := by
   induction t with
-  | nil => grind[complete, del]
+  | nil => grind[ del]
   | node2 l a r l_ih r_ih =>
-      grind[completeness_preservation_deleteTree_node21, completeness_preservation_deleteTree_node22, complete_deleteHeight, complete,  splitMin_height_complete, splitMin_complete, deleteTree, del]
+      grind[completeness_preservation_deleteTree_node21, completeness_preservation_deleteTree_node22, complete_deleteHeight, splitMin_height_complete, splitMin_complete, del]
   | node3 l a m b r l_ih m_ih r_ih =>
-      grind[completeness_preservation_deleteTree_node31, completeness_preservation_deleteTree_node32, completeness_preservation_deleteTree_node33, complete_deleteHeight, complete, splitMin_height_complete, splitMin_complete, deleteTree, del]
+      grind[completeness_preservation_deleteTree_node31, completeness_preservation_deleteTree_node32, completeness_preservation_deleteTree_node33, complete_deleteHeight, splitMin_height_complete, splitMin_complete, del]
 
 lemma delete_completeness_preservation (t : Tree23 α) (x : α) (h : complete t):
     complete (delete x t h) := by
@@ -398,7 +389,7 @@ lemma node22_preserves_members
   (hx : ∀ x: α, x ∈ setTree (deleteTree r_up) → x ∈ setTree r):
     el ∈ setTree (deleteTree (node22 l a r_up hl)) → el ∈ setTree (node2 l a r) := by
   cases req : r_up
-  · grind[node22]
+  · grind
   · simp[node22]
     cases l <;> grind
 
@@ -462,7 +453,7 @@ lemma splitMin_preserves_members
     · grind
     · rename_i hnn
       simp
-      specialize l_ih (by grind[complete]) (by grind)
+      specialize l_ih (by grind  ) (by grind)
       intro h'
       cases h'
       · specialize l_ih el
@@ -492,8 +483,8 @@ lemma del_preserves_members (x : α ) (t : Tree23 α) (ht : complete t) (y : α 
   induction t generalizing y with
   | nil => grind
   | node2 l a r l_ih r_ih =>
-    specialize l_ih (by grind[complete])
-    specialize r_ih (by grind[complete])
+    specialize l_ih (by grind  )
+    specialize r_ih (by grind  )
     unfold del at h
     split at h
     · split at h
@@ -501,8 +492,8 @@ lemma del_preserves_members (x : α ) (t : Tree23 α) (ht : complete t) (y : α 
       · grind
     · split at h
       · cases del_eq : (del x l (by grind : complete l))
-        · grind[node21]
-        · simp [del_eq, deleteTree, node21] at h
+        · grind
+        · simp [del_eq, node21] at h
           cases r <;> grind
       · split at h
         · have : y ∈ setTree (deleteTree (node22
@@ -515,13 +506,13 @@ lemma del_preserves_members (x : α ) (t : Tree23 α) (ht : complete t) (y : α 
             grind[node22_preserves_members]
           grind
         · cases del_eq : (del x r (by grind : complete r))
-          · grind[node22]
+          · grind
           · simp [del_eq, deleteTree, node22] at h -- grind needs simp here
             grind
   | node3 l a m b r l_ih m_ih r_ih =>
-    specialize l_ih (by grind[complete])
-    specialize m_ih (by grind[complete])
-    specialize r_ih (by grind[complete])
+    specialize l_ih (by grind  )
+    specialize m_ih (by grind  )
+    specialize r_ih (by grind  )
     unfold del at h
     split at h
     · split at h <;> grind
@@ -557,7 +548,7 @@ lemma del_preserves_members (x : α ) (t : Tree23 α) (ht : complete t) (y : α 
 lemma searchTree_node21_searchTree (l' : DeleteUp α) (r : Tree23 α) (a : α) (h1: searchTree (deleteTree l')) (h2: searchTree r) (h3: ∀ x ∈ setTree (deleteTree l'), x < a) (h4: ∀ x ∈ setTree r, a < x) (hrn : r ≠ nil):
   searchTree (deleteTree (node21 l' a r hrn)) := by
   induction l' with
-  | eq l' => grind[node21]
+  | eq l' => grind
   | underflow l' =>
     simp[node21]
     cases r with
@@ -571,31 +562,29 @@ lemma searchTree_node21_searchTree (l' : DeleteUp α) (r : Tree23 α) (a : α) (
 lemma searchTree_node22_searchTree (r': DeleteUp α) (l : Tree23 α) (a : α) (h1: searchTree (deleteTree r')) (h2: searchTree l) (h3: ∀ x ∈ setTree (deleteTree r'), a < x) (h4: ∀ x ∈ setTree l, x < a) (hln : l ≠ nil):
   searchTree (deleteTree (node22 l a r' hln)) := by
   induction r' with
-  | eq r' =>
-    grind[node22]
+  | eq r' => grind
   | underflow r' =>
     simp[node22]
     cases l with
     | nil => grind
     | node2 l a r => grind
     | node3 l a' m b r =>
-      have : a > b := by grind[setTree]
+      have : a > b := by grind
       grind
 
 
 lemma searchTree_node31_searchTree (l' : DeleteUp α) (m : Tree23 α) (r : Tree23 α) (a : α) (b : α) (hsl': searchTree (deleteTree l')) (hsm: searchTree m) (hsr: searchTree r) (hab : a < b) (hl's: ∀ x ∈ setTree (deleteTree l'), x < a) (hms: ∀ x ∈ setTree m, a < x) (hmb: ∀ x ∈ setTree m, x < b) (hrs: ∀ x ∈ setTree r, b < x) (hmn : m ≠ nil) (hrn : r ≠ nil) :
     searchTree (deleteTree (node31 l' a m b r hmn hrn)) := by
   induction l' with
-  | eq l' => grind[node31]
+  | eq l' => grind
   | underflow l' =>
-    simp[node31]
     cases m <;> grind
 
 
 lemma searchTree_node32_searchTree (m' : DeleteUp α) (l : Tree23 α) (r : Tree23 α) (a : α) (b : α) (hsm': searchTree (deleteTree m')) (hsl: searchTree l) (hsr: searchTree r) (hab : a < b) (hm's :  ∀ x ∈ setTree (deleteTree m'), a < x) (hm'b : ∀ x ∈ setTree (deleteTree m'), x < b) (hrs: ∀ x ∈ setTree r, b < x) (hls: ∀ x ∈ setTree l, x < a) (hln : l ≠ nil) (hrn : r ≠ nil) :
     searchTree (deleteTree (node32 l a m' b r hln hrn)) := by
   induction m' with
-  | eq m' => grind[node32]
+  | eq m' => grind
   | underflow m' =>
     simp[node32]
     cases r with
@@ -610,9 +599,8 @@ lemma searchTree_node32_searchTree (m' : DeleteUp α) (l : Tree23 α) (r : Tree2
 lemma searchTree_node33_searchTree (r' : DeleteUp α) (l : Tree23 α) (m : Tree23 α) (a : α) (b : α) (hsr': searchTree (deleteTree r')) (hsl: searchTree l) (hsm: searchTree m) (hab : a < b) (hr's: ∀ x ∈ setTree (deleteTree r'), b < x) (hms: ∀ x ∈ setTree m, a < x) (hmb: ∀ x ∈ setTree m, x < b) (hls: ∀ x ∈ setTree l, x < a) (hln : l ≠ nil) (hmn : m ≠ nil) :
     searchTree (deleteTree (node33 l a m b r' hln hmn)) := by
   induction r' with
-  | eq r' => grind[node33]
+  | eq r' => grind
   | underflow r' =>
-    simp[node33]
     cases m <;> grind
 
 
@@ -684,7 +672,7 @@ lemma searchTree_del_searchTree (t: Tree23 α) (x: α) (h: complete t):
     searchTree t → searchTree (deleteTree (del x t h)) := by
   intro hsT
   induction t with
-  | nil => grind[searchTree, del]
+  | nil => grind[del]
   | node2 l a r l_ih r_ih =>
       obtain ⟨ hl, hr, hl', hr' ⟩ := hsT
       specialize l_ih (by grind) hl'
@@ -709,7 +697,7 @@ lemma searchTree_del_searchTree (t: Tree23 α) (x: α) (h: complete t):
             · assumption
             · grind[deleteTree_splitMin_preserves_searchTree_1]
             · intro x' hx
-              have h1 : (r.splitMin (by grind[complete]) (by grind[complete])).1 ∈ r.setTree := by grind
+              have h1 : (r.splitMin (by grind  ) (by grind  )).1 ∈ r.setTree := by grind
               grind
           · expose_names;
             apply searchTree_node22_searchTree
@@ -722,9 +710,9 @@ lemma searchTree_del_searchTree (t: Tree23 α) (x: α) (h: complete t):
             · assumption
   | node3 l a m b r l_ih m_ih r_ih =>
       obtain ⟨ hab, hl, hma, hmb, hr, hl', hm', hr' ⟩ := hsT
-      specialize l_ih (by grind[complete]) hl'
-      specialize m_ih (by grind[complete]) hm'
-      specialize r_ih (by grind[complete]) hr'
+      specialize l_ih (by grind  ) hl'
+      specialize m_ih (by grind  ) hm'
+      specialize r_ih (by grind  ) hr'
       unfold del
       split
       · grind
@@ -739,7 +727,7 @@ lemma searchTree_del_searchTree (t: Tree23 α) (x: α) (h: complete t):
             · grind[deleteTree_splitMin_preserves_searchTree_1]
             · grind
             · assumption
-            · have : (m.splitMin (by grind) (by grind[complete])).1 ∈ m.setTree := by
+            · have : (m.splitMin (by grind) (by grind  )).1 ∈ m.setTree := by
                 grind
               grind
           · split
@@ -749,12 +737,12 @@ lemma searchTree_del_searchTree (t: Tree23 α) (x: α) (h: complete t):
                 · grind[deleteTree_splitMin_preserves_searchTree_2]
                 · assumption
                 · assumption
-                · have : (r.splitMin (by grind) (by grind[complete])).1 ∈ r.setTree := by
+                · have : (r.splitMin (by grind) (by grind  )).1 ∈ r.setTree := by
                     grind
                   grind
                 · grind[deleteTree_splitMin_preserves_searchTree_1]
                 · assumption
-                · have : (r.splitMin (by grind) (by grind[complete])).1 ∈ r.setTree := by
+                · have : (r.splitMin (by grind) (by grind  )).1 ∈ r.setTree := by
                     grind
                   grind
                 · assumption
